src/Parsers/MinimalParse.v
@@ -11,7 +11,7 @@ Local Open Scope string_like_scope.
 Section cfg.
   Context {Char} {HSL : StringLike Char} {G : grammar Char}.
   Context {predata : @parser_computational_predataT}
-          {rdata' : @parser_removal_dataT' predata}.
+          {rdata' : @parser_removal_dataT' _ G predata}.
 
   (** The [nonterminals_listT] is the current list of valid nonterminals to compare
       against; the extra [String] argument to some of these is the
