src/Parsers/Reachable/MaybeEmpty/OfParse.v
@@ -18,7 +18,7 @@ Local Open Scope string_like_scope.
 Section cfg.
   Context {Char} {HSL : StringLike Char} {HSLP : StringLikeProperties Char} {G : grammar Char}.
   Context {predata : parser_computational_predataT}
-          {rdata' : @parser_removal_dataT' predata}.
+          {rdata' : @parser_removal_dataT' _ G predata}.
 
   Definition parse_empty_maybe_empty_parse_of_item'
              (parse_empty_maybe_empty_parse_of_productions
