src/Parsers/Reachable/ParenBalancedHiding/MinimalOfCore.v
@@ -16,7 +16,7 @@ Local Open Scope string_like_scope.
 Section cfg.
   Context {Char} {HSL : StringLike Char} {HSLP : StringLikeProperties Char} {G : grammar Char}.
   Context {predata : parser_computational_predataT}
-          {rdata' : @parser_removal_dataT' predata}
+          {rdata' : @parser_removal_dataT' _ G predata}
           {pdata : paren_balanced_hiding_dataT Char}.
 
   Local Arguments pbh'_production / .
